\documentclass[a4paper,12pt]{article}

\usepackage{amssymb}
\usepackage{amsmath}
\usepackage{amsthm}
\usepackage[hmargin=25mm]{geometry}
\usepackage{graphicx}
\usepackage[hidelinks]{hyperref}
\usepackage[utf8]{inputenc}

\newtheorem{theorem}[equation]{Theorem}
\newtheorem{assumption}[equation]{Assumption}
\newtheorem{corollary}[equation]{Corollary}
\newtheorem{conjecture}[equation]{Conjecture}
\newtheorem{lemma}[equation]{Lemma}
\newtheorem{proposition}[equation]{Proposition}
\theoremstyle{definition}
\newtheorem{definition}[equation]{Definition}

\newcommand{\dd}{\mathrm{d}}
\newcommand{\C}{\mathcal{C}}
\newcommand{\D}{\mathcal{D}}
\newcommand{\E}{\mathbb{E}}
% \newcommand{\I}{1\!\!\!\;\mathrm{I}}
\renewcommand{\P}{\mathbb{P}}
\newcommand{\R}{\mathbb{R}}
\newcommand{\V}{\mathbb{V}}
\newcommand{\Z}{\mathbb{Z}}

\newcommand{\ind}{\perp\mkern-10mu\perp}

\renewcommand{\geq}{\geqslant}
\renewcommand{\leq}{\leqslant}
\renewcommand{\ge}{\geqslant}
\renewcommand{\le}{\leqslant}

\setlength{\parindent}{0pt}
\setlength{\parskip}{.6em}
\renewcommand{\baselinestretch}{1.15}

\usepackage{embedall}

\begin{document}

\title{Lyapunov's Central Limit Theorem}
\author{Leonardo T. Rolla}
\date{June 1, 2017}
\maketitle

{\let\thefootnote\relax
\footnotetext{\copyright 2017-\the\year\ Leonardo T. Rolla
\href{http://creativecommons.org/licenses/by-sa/3.0/}
{\includegraphics[height=1.0em]{by-sa.pdf}}. This typeset file has the source code embedded in it. If you re-use part of this code, you are kindly requested --if possible-- to convey the source code along with or embedded in the typeset file, and to keep this request.}}

\begin{theorem}
% [De~Moivre 1730, Laplace 1812]
Let $(X_n)_n$ be independent with finite third moments such that
\[
\frac{\sum_{i=1}^{n} E|X_i-EX_i|^3}{\left( \sum_{i=1}^{n} VX_i \right)^{3/2}} \to 0
\text{ as }
n\to \infty
.
\]
Then,
\[
E f\left( \frac{S_n-ES_n}{\sqrt{VS_n}} \right) \to \int_\R f(x) \frac{e^{-x^2/2}}{\sqrt{2\pi}} \dd x
\text{ as }
n\to \infty
\]
for any $f$ such that $f$, $f'$, $f''$ and $f'''$ are bounded.
\end{theorem}

% Remark.
It turns out, convergence for all $f$ satisfying these conditions is equivalent to convergence for all bounded continuous $f$, which is equivalent to convergence in distribution.

\section*{Proof}

We can assume $EX_i=0$ without loss of generality.
Write $\sigma_i = \sqrt{VX_i}$.
Consider $(Y_n)_n$ independent, and also independent of $(X_n)_n$, with distribution $\mathcal{N}(0,\sigma_i^2)$.
\\{}
[We accept without proof existence of such sequence in the same probability space.]

Write
\[
W_n
=
\frac{Y_1+\dots+Y_n}{\sqrt{VS_n}}
\sim
\mathcal{N}(0,1)
\quad
\text{ and }
\quad
Z_n
=
\frac{X_1+\dots+X_n}{\sqrt{VS_n}}
.
\]
Fix $n$, define $Z^0 = W_n$ and, for $i=1,\dots,n$, define
\[
V^i = Z^{i-1} - \frac{Y_i}{\sqrt{VS_n}}
\quad
\text{ and }
\quad
Z^i = V^{i} + \frac{X_i}{\sqrt{VS_n}},
\]
so that $Z^n = Z_n$.
Now,
\[
Ef(Z_n) - Ef(W_n)
=
Ef(Z^n) - Ef(Z^0)
=
\sum_{i=1}^n
Ef(Z^i)-Ef(Z^{i-1})
.
\]
Using the Taylor expansion of $f$,
\begin{align*}
f(Z^i)
=
f(V_i+\frac{X_i}{\sqrt{VS_n}})
& =
f(V^i) + f'(V^i) \frac{X_i}{\sqrt{VS_n}} + \frac{f''(V_i)}{2}\frac{X_i^2}{{VS_n}} + \frac{f'''(\theta^i)}{6}\frac{X_i^3}{(VS_n)^{3/2}}
,
\\
f(Z^{i-1})
=
f(V_i+\frac{Y_i}{\sqrt{VS_n}})
& =
f(V^i) + f'(V^i) \frac{Y_i}{\sqrt{VS_n}} + \frac{f''(V_i)}{2}\frac{Y_i^2}{{VS_n}} + \frac{f'''(\tilde\theta^i)}{6}\frac{Y_i^3}{(VS_n)^{3/2}}
,
\end{align*}
where $\theta_i$ and $\tilde\theta_i$ come from the Taylor polynomial and depend on $V_i$, $X_i$ and $Y_i$.

Notice that $EX_i=EY_i$, $EX_i^2=EY_i^2$, $X_i \ind V^i$ and $Y_i \ind V^i$, and recall that $f$ and its first three derivatives are bounded.
We want to take expectation above and subtract. Since $f$ is bounded, $f(V^i)$ is integrable and this first term cancels out.
Also, $f'(V^i)$ is integrable and, by independence,
\[
E[f'(V^i) X_i] = Ef'(V^i) \cdot EX_i = Ef'(V^i) \cdot EY_i = E[f'(V^i) Y_i],
\]
so this term also cancels out, as well as the third one for the same reason.
Thus,
\[
Ef(Z^i) - Ef(Z^{i-1}) = \frac{E[f'''(\theta_i){X_i^3}] - E[f'''(\tilde\theta_i)Y_i^3]}{6({VS_n})^{3/2}}
,
\]
so taking $C=\sup_x |f'''(x)|$ we get
\begin{align*}
\left| \big. Ef(Z^i)-Ef(Z^{i-1}) \right|
& \leq
\frac{C E|X_i|^3 + CE|Y_i|^3}{6({VS_n})^{3/2}}
\\
& =
C \frac{ E|X_i|^3 + \sigma_i^3 E|\mathcal{N}|^3 }{6({VS_n})^{3/2}}
\\
& \leq
C \frac{ E|X_i|^3 }{({VS_n})^{3/2}}
,
\end{align*}
where in the last inequality we used that $E|\mathcal{N}|^3 = \frac{4}{\sqrt{2\pi}} < 2$ and that
\[
\sigma_i = (E|X_i|^2)^{\frac{1}{2}} \leq (E|X_i|^3)^{\frac{1}{3}}
\]
by Jensen's inequality.
Finally, summing over $i$,
\[
\left| \big. Ef(Z^i)-Ef(Z^{i-1}) \right|
\le
\sum_{i=1}^n
\left| \big. Ef(Z^i)-Ef(Z^{i-1}) \right|
\le
C
\frac{\sum_{i=1}^{n} E|X_i|^3}{\left( \sum_{i=1}^{n} VX_i \right)^{3/2}} \to 0
\]
as
$n\to \infty$
by assumption,
concluding the proof of the theorem.

\end{document}
